AlgoleanTests.lean
@@ -3,6 +3,7 @@ module  -- shake: keep-all --deprecated_module: ignore
 public import AlgoleanTests.CircuitExamples
 public import AlgoleanTests.FreeMonadWP
 public import AlgoleanTests.KMPExamples
+public import AlgoleanTests.ModelMWP
 public import AlgoleanTests.NaivePatternSearchExamples
 public import AlgoleanTests.ProgExamples
 public import AlgoleanTests.QueryExamples
